Initial commit

history.fst
@@ -1,146 +1,70 @@
 module History
 
-open FStar.List.Tot
-
 module L = FStar.List.Tot
 
-module Vc = Vector_clock
+module I = Icounter
 
 type state = nat
 
 type history (n:nat) =
-| History : clock:Vc.t n
-          -> state:state
-          -> children:list (history n)
-          -> history n
+| History : state:state
+            -> children:list (I.trace * history n)
+            -> history n
 
-val wellformed : #n:nat -> h:history n -> Tot bool (decreases %[h])
-val wellformed' : #n:nat -> l:list (history n) -> parent_clock:Vc.t n -> Tot bool (decreases %[l])
-let rec wellformed h =
-  let History clock _ ch = h in
-  wellformed' ch clock
-and wellformed' children parent_clock =
+
+val hbeq : #n:nat -> h1:history n -> h2:history n -> Tot bool (decreases %[h1]) 
+val hbeq' : #n:nat -> l:list (I.trace * history n) -> h2:history n -> Tot bool (decreases %[l])
+let rec hbeq #n h1 h2 =
+  let History s ch = h1 in 
+  h1 = h2 || hbeq' #n ch h2 
+and hbeq' #n children h2 =
   match children with
-  | [] -> true
-  | x::xs ->
-     let clock = History?.clock x in
-     Vc.hb parent_clock clock &&
-     wellformed x &&
-     wellformed' xs parent_clock
-     
-val mem : #n:nat -> clock:Vc.t n -> h:history n -> Tot bool (decreases %[h])
-val mem' : #n:nat -> l:list (history n) -> clock:Vc.t n -> Tot bool (decreases %[l])
-let rec mem clock h = 
-  let History k _ ch = h in
-  clock = k || mem' ch clock
-and mem' l clock = 
-  match l with
-  | [] -> false
-  | x::xs -> mem clock x || mem' xs clock
+  |[] -> false
+  |(tr,x)::xs -> hbeq #n x h2 || hbeq' #n xs h2
+  
 
+val eq : #n:nat -> h1:history n -> h2:history n -> Tot bool (decreases %[h1]) 
+let eq #n h1 h2 = (h1 = h2)
+
+val hb : #n:nat -> h1:history n -> h2:history n -> Tot bool (decreases %[h1])
+let hb #n h1 h2 = hbeq h1 h2 && not(eq h1 h2)
+          
 
 val size : #n:nat -> h:history n -> Tot nat (decreases %[h])
-val size' : #n:nat -> l:list (history n) -> Tot nat (decreases %[l])
-let rec size h =
-  let History _ _ ch = h in
-  1 + size' ch
-and size' l = 
-  match l with
-  | [] -> 0
-  | x::xs -> size x + size' xs
+val size' : #n:nat -> l:list (I.trace * history n) -> Tot nat (decreases %[l])
+let rec size #n h =
+    let History  _ ch = h in
+    1 + size' ch
+and size' #n l = 
+    match l with
+    | [] -> 0
+    | (tr,x)::xs -> size x + size' xs
+    
 
-val lemma1 : #n:nat -> h:history n{wellformed h}
-           -> Lemma (ensures (forall h'. L.mem h' (History?.children h) ==> wellformed h')) (decreases (size h))
-let rec lemma1 (History c s ch) =
-  match ch with
-  | [] -> ()
-  | x::xs -> assert (wellformed x); lemma1 (History c s xs)
+val wellformed : #n:nat -> h:history n -> Tot bool (decreases %[h])
+val wellformed' : #n:nat -> s:state -> l:list (I.trace * history n) -> h:history n -> Tot bool (decreases %[l])
+let rec wellformed #n h =
+  let History state ch = h in
+  wellformed' state ch h
+and wellformed' #n parent_state children parent_history =
+  match children with
+  |[] -> true
+  |(tr,child_history)::xs -> 
+    let state = History?.state child_history in
+    state = I.apply_tr tr parent_state &&
+    hb parent_history child_history &&
+    wellformed child_history &&
+    wellformed' parent_state xs parent_history
 
-val lemma2 : #n:nat -> h:history n{wellformed h}
-           -> Lemma (ensures (forall c. mem c h ==> Vc.hbeq (History?.clock h) c)) (decreases (size h))
-val lemma2' : #n:nat -> h:history n{wellformed h} -> c:Vc.t n{Vc.hbeq c (History?.clock h)}
-           -> Lemma (requires (forall k. mem k h ==> Vc.hbeq (History?.clock h) k))
-                   (ensures  (forall k. mem k h ==> Vc.hbeq c k)) (decreases (size h))
-let rec lemma2 h =
-  let History c s ch = h in
-  match ch with
-  | [] -> Vc.hbeq_reflexive c
-  | x::xs ->
-      lemma2 x;
-      lemma2 (History c s xs);
-      assert (Vc.hbeq c (History?.clock x));
-      assert (forall k. mem k x ==> Vc.hbeq (History?.clock x) k);
-      lemma2' x c;
-      assert (forall k. mem k x ==> Vc.hbeq c k);
-      ()
-and lemma2' (History c' s ch) c =
-  match ch with
-  | [] -> ()
-  | x::xs -> 
-      Vc.hbeq_transitive (length c) c c' (History?.clock x);
-      lemma2 x;
-      lemma2' x c;
-      lemma2 (History c' s xs);
-      lemma2' (History c' s xs) c;
-      ()
+val test : #n:nat -> Tot unit
+let test #n = assert (hbeq #n (History 1 [([I.Inc;I.Inc], (History 3 [([I.Inc],(History 4 []))]))]) (History 3 [([I.Inc],(History 4 []))]));()
 
-val append : #n:nat -> p:(Vc.t n -> bool) 
-           -> l1:list (Vc.t n){forall e. L.mem e l1 ==> p e}
-           -> l2:list (Vc.t n){forall e. L.mem e l2 ==> p e}
-           -> l:list (Vc.t n){forall e. L.mem e l ==> p e}
-let rec append p l1 l2 =
-  match l1 with
-  | [] -> l2
-  | x::xs -> x::(append p xs l2)
+val test1 : #n:nat -> Tot unit
+let test1 #n = assert (hb #n (History 1 [([I.Inc;I.Inc], (History 3 [([I.Inc],(History 4 []))]))]) (History 4 []));()
 
-val is_concurrent : #n:nat -> v:Vc.t n -> l:list (Vc.t n) 
-                  -> r:bool{(forall c. L.mem c l ==> (v = c \/ Vc.concurrent v c)) <==> r = true}
-let rec is_concurrent v l =
-  match l with
-  | [] -> true
-  | x::xs -> (v = x || Vc.concurrent v x) && is_concurrent v xs
+val test2 : #n:nat -> Tot unit
+let test2 #n = assert (eq #n (History 1 [([I.Inc;I.Inc], (History 3 [([I.Inc],(History 4 []))]))]) (History 1 [([I.Inc;I.Inc], (History 3 [([I.Inc],(History 4 []))]))]));()
 
-val cross_concurrent : #n:nat -> l:list (Vc.t n) 
-                     -> r:list (Vc.t n){(forall c. L.mem c r ==> L.mem c l) /\ 
-                                       (forall c1 c2. L.mem c1 r /\ L.mem c2 r ==> c1 = c2 \/ Vc.concurrent c1 c2)}
-let rec cross_concurrent l1 =
-  match l1 with
-  | [] -> []
-  | x::xs -> 
-      if is_concurrent x xs then begin
-        x::(cross_concurrent xs)
-      end else cross_concurrent xs 
 
-val get_latest : #n:nat -> p:(Vc.t n -> bool)
-               -> l:list (Vc.t n){forall c. L.mem c l ==> p c}
-               -> l':list (Vc.t n){(forall c. L.mem c l' ==> L.mem c l /\ p c)}
-let get_latest p l = cross_concurrent l
 
-val lca : #n:nat -> h:history n{wellformed h} -> a:Vc.t n{mem a h} -> b:Vc.t n{mem b h}
-        -> Tot (lcalst:list (Vc.t n){(forall l. L.mem l lcalst ==> mem l h /\ Vc.hbeq l a /\ Vc.hbeq l b) /\
-                                    (forall c1 c2. L.mem c1 lcalst /\ L.mem c2 lcalst ==> c1 = c2 \/ Vc.concurrent c1 c2)}) (decreases (size h))
-let rec lca h a b =
-  lemma2 h;
-  let History c s ch = h in
-  match ch with
-  | [] -> [c]
-  | x::xs ->
-      let l1 =
-        if mem a x && mem b x then
-            lca x a b
-        else []
-      in
-      let h' = History c s xs in
-      let l2 =
-        if mem a h' && mem b h' then
-            lca h' a b
-        else []
-      in
-      assert (forall c. L.mem c l1 ==> mem c h /\ Vc.hbeq c a /\ Vc.hbeq c b);
-      assert (forall c. L.mem c l2 ==> mem c h /\ Vc.hbeq c a /\ Vc.hbeq c b);
-      assert (mem c h /\ Vc.hbeq c a /\ Vc.hbeq c b);
-      let l = (c::(l1@l2)) in
-      let p = fun c -> mem c h && Vc.hbeq c a && Vc.hbeq c b in
-      let l = c::(append p l1 l2) in
-      assert (forall c. L.mem c l ==> mem c h /\ Vc.hbeq c a /\ Vc.hbeq c b);
-      get_latest p l
+
