icounter.fst
@@ -1,90 +1,25 @@
-module ICounter
+module Icounter
 
 open FStar.List.Tot
 
-type state = nat
+module L = FStar.List.Tot
+
+module H = History
 
 type operation =
   | Inc : nat -> operation
 
 type trace = list operation
 
-val apply_op : operation -> state -> nat
-let apply_op (Inc n) s = s + n
+val apply_op : operation -> s1:H.state -> s2:H.state {s2 >= s1} 
+let apply_op op s = 
+  match op with
+  | Inc n -> s + n
 
+val apply_tr : t:trace -> s1:H.state -> s2:H.state {s2 >= s1}
 let rec apply_tr t s =
   match t with
   | [] -> s
   | op::ops -> apply_tr ops (apply_op op s)
 
-val lem_trans : a:state
-           -> t0:trace
-           -> b:state{apply_tr t0 a = b}
-           -> t1:trace
-           -> c:state{apply_tr t1 b = c}
-           -> Lemma (ensures (apply_tr (append t0 t1) a = c)) (decreases %[t0;t1])
-let rec lem_trans a t0 b t1 c = match t0 with
-| [] -> ()
-| op::ops -> lem_trans (apply_op op a) ops b t1 c
 
-val concat_trace : a:state
-                -> t0:trace
-                -> b:state{apply_tr t0 a = b}
-                -> t1:trace
-                -> c:state{apply_tr t1 b = c}
-                -> t:trace{t = append t0 t1 /\ apply_tr t a = c}
-let concat_trace a t0 b t1 c = 
-  lem_trans a t0 b t1 c;
-  append t0 t1
-
-val lem_monotonic_increase : t:trace 
-                           -> inp:state 
-                           -> Lemma (ensures (apply_tr t inp >= inp))
-let rec lem_monotonic_increase t inp = 
-  match t with
-  | [] -> ()
-  | op::ops -> lem_monotonic_increase ops (apply_op op inp)
-
-val merge_trace : lca:state
-                -> t0:trace
-                -> a:state{apply_tr t0 lca = a}
-                -> t1:trace
-                -> b:state{apply_tr t1 lca = b}
-                -> trace
-let merge_trace lca t0 a t1 b =
-  lem_monotonic_increase t0 lca;
-  lem_monotonic_increase t1 lca;
-  [Inc (a - lca + b - lca)]
-
-val merge : lca:state
-          -> t0:list operation
-          -> a:state{apply_tr t0 lca = a}
-          -> t1:list operation
-          -> b:state{apply_tr t1 lca = b}
-          -> m:state{m = apply_tr (merge_trace lca t0 a t1 b) lca}
-let merge lca t0 a t1 b =
-  lem_monotonic_increase t0 lca;
-  assert(a >= lca);
-  a + b - lca
-
-val commutativity : lca:state
-                  -> t0:list operation
-                  -> a:state{apply_tr t0 lca = a}
-                  -> t1:list operation
-                  -> b:state{apply_tr t1 lca = b}
-                  -> Lemma (ensures (merge lca t0 a t1 b) = (merge lca t1 b t0 a))
-let commutativity lca t0 a t1 b = ()
-
-
-val associativity : l0:state
-                  -> t0:list operation
-                  -> l1:state{apply_tr t0 l0 = l1}
-                  -> t1:list operation
-                  -> a:state{apply_tr t1 l1 = a}
-                  -> t2:list operation
-                  -> b:state{apply_tr t2 l1 = b}
-                  -> t3:list operation
-                  -> c:state{apply_tr t3 l0 = c}
-                  -> Lemma (ensures (merge l0 (concat_trace l0 t0 l1 (merge_trace l1 t1 a t2 b) (merge l1 t1 a t2 b)) (merge l1 t1 a t2 b) t3 c =
-                                    merge l1 t1 a (merge_trace l0 (concat_trace l0 t0 l1 t2 b) b t3 c) (merge l0 (concat_trace l0 t0 l1 t2 b) b t3 c)))
-let associativity l0 t0 l1 t1 a t2 b t3 c = ()
